crypto.v
@@ -10,83 +10,9 @@ From iris.base_logic.lib Require Import invariants.
 From iris_string_ident Require Import ltac2_string_ident.
 From crypto Require Import basic.
 
-Section Keys.
-
-Class key2SG Σ := KeySG {
-  key_inG :> inG Σ (authR (gsetUR (prodO locO locO)));
-  key2_symbol : gname;
-  key1_symbol : gname;
-  key_name : gname;
-}.
-
-Context `{symbolSG Σ, keySG Σ}.
-
-Implicit Types LL : gsetUR (prodO locO locO).
-Implicit Types ll : prodO locO locO.
-Implicit Types Lb : gsetUR (prodO boolO locO).
-Implicit Types l : locO.
-
-Definition key_inv : iProp Σ :=
-  ∃ LL,
-    own key_name (● LL) ∗
-    ⌜perm LL⌝ ∗
-    ([∗ set] ll ∈ LL, symbol true  key2_symbol ll.1 ∗
-                      symbol false key2_symbol ll.2).
-
-Definition key l1 l2 : iProp Σ :=
-  own key_name (◯ {[l1, l2]}).
-
-Global Instance key_persistent l1 l2 : Persistent (key l1 l2).
-Proof. apply _. Qed.
-
-Lemma key_permR l1 l21 l22 :
-  key_inv -∗ key l1 l21 -∗ key l1 l22 -∗ ⌜l21 = l22⌝.
-Proof.
-iDestruct 1 as (LL) "(Hown & %Hperm & Halloc)".
-iIntros "Hl21 Hl22"; rewrite /key.
-iPoseProof (own_valid_2 with "Hown Hl21") as "%Hvalid1".
-rewrite auth_both_valid in Hvalid1 *; case=> Hvalid1 _.
-iPoseProof (own_valid_2 with "Hown Hl22") as "%Hvalid2".
-rewrite auth_both_valid in Hvalid2 *; case=> Hvalid2 _.
-have {}Hvalid1: (l1, l21) ∈ LL.
-  move/gset_included in Hvalid1; apply: Hvalid1.
-  by apply elem_of_singleton_2.
-have {}Hvalid2: (l1, l22) ∈ LL.
-  move/gset_included in Hvalid2; apply: Hvalid2.
-  by apply elem_of_singleton_2.
-by iPureIntro; apply (Hperm _ _ Hvalid1 Hvalid2).
-Qed.
-
-Lemma key_permL l11 l12 l2 :
-  key_inv -∗ key l11 l2 -∗ key l12 l2 -∗ ⌜l11 = l12⌝.
-Proof.
-iDestruct 1 as (LL) "(Hown & %Hperm & Halloc)".
-rewrite /key; iIntros "Hl11 Hl12".
-iPoseProof (own_valid_2 with "Hown Hl11") as "%Hvalid1".
-iPoseProof (own_valid_2 with "Hown Hl12") as "%Hvalid2".
-move: Hvalid1; rewrite auth_both_valid; case=> Hvalid1 _.
-move: Hvalid2; rewrite auth_both_valid; case=> Hvalid2 _.
-have {}Hvalid1 : (l11, l2) ∈ LL.
-  move/gset_included in Hvalid1; apply: Hvalid1.
-  by apply elem_of_singleton_2.
-have {}Hvalid2 : (l12, l2) ∈ LL.
-  move/gset_included in Hvalid2; apply: Hvalid2.
-  by apply elem_of_singleton_2.
-by iPureIntro; apply (Hperm _ _ Hvalid1 Hvalid2).
-Qed.
-
-End Keys.
-
 Section Terms.
 
-Context `{heapG Σ, cfgSG Σ, symbolSG Σ}.
-
-Implicit Types s : side.
-
-Definition lo_nonce : symbol_kind := 1%positive.
-Definition hi_nonce : symbol_kind := 2%positive.
-Definition lo_key   : symbol_kind := 3%positive.
-Definition hi_key   : symbol_kind := 4%positive.
+Context `{heapG Σ, cfgSG Σ, symbolSG Σ, symbol2SG Σ}.
 
 Inductive term  :=
 | TInt of Z
@@ -104,15 +30,19 @@ Fixpoint val_of_term t : val :=
   | TEnc l t => (#4, (#l, val_of_term t))
   end.
 
-
 Class termSG := TermSG {
-  term_inG  :> inG Σ (authR (gsetUR (prodO valO valO)));
-  term_name :  gname
+  term_inG    :> inG Σ (authR (gsetUR (prodO valO valO)));
+  key_name    :  gname;
+  key2_name   :  gname;
+  nonce_name  :  gname;
+  nonce2_name :  gname;
+  term_name   :  gname;
 }.
 
-Section Terms.
-
 Context `{termSG}.
+
+
+
 
 Fixpoint opaque s t : iProp Σ :=
   match t with
